examples/algorithms/qsc.fst
@@ -1,3 +1,7 @@
+(*--build-config
+    options:--admit_fsi Set --z3timeout 20;
+    other-files:set.fsi heap.fst st.fst all.fst list.fst
+  --*)
 module QuickSort
 open List
 #set-options "--initial_ifuel 2 --initial_fuel 1 --max_ifuel 2 --max_fuel 1"
