examples/unit-tests/mac2.fst
@@ -1,3 +1,7 @@
+(*--build-config
+    options:--admit_fsi Set --admit_fsi Seq --admit_fsi SeqProperties;
+    other-files:classical.fst ext.fst set.fsi heap.fst st.fst all.fst seq.fsi list.fst
+  --*)
 (*
    Copyright 2008-2014 Nikhil Swamy and Microsoft Research
 
@@ -18,37 +22,36 @@
    hashes, namely HMAC-SHA1, and their idealization under the INT-CMA
    computational assumption *)
 
-module MAC 
-
-open Array
-type bytes = seq byte (* concrete byte arrays *) 
+module MAC
+open Seq
+type bytes = seq byte (* concrete byte arrays *)
 type text  = bytes    (* a type abbreviation, for clarity *)
 
 type nbytes (n:nat) = b:bytes{length b = n} (* fixed-length bytes *)
 
-let keysize = 16 (* these are the sizes for SHA1 *) 
-let macsize = 20  
+let keysize = 16 (* these are the sizes for SHA1 *)
+let macsize = 20
 type key = nbytes keysize
 type tag = nbytes macsize
 
 (* we rely on some external crypto library implementing HMAC-SHA1 *)
 
-assume val sha1: key -> text -> Tot tag 
+assume val sha1: key -> text -> Tot tag
 
-(* to verify, we simply recompute & compare *) 
+(* to verify, we simply recompute & compare *)
 
 val sha1verify: key -> text -> tag -> Tot bool
 let sha1verify k txt tag = (sha1 k txt = tag)
 
-(* we attach an authenticated properties to each key, 
-   used as a pre-condition for MACing and 
+(* we attach an authenticated properties to each key,
+   used as a pre-condition for MACing and
    a postcondition of MAC verification *)
 
 opaque type key_prop : key -> text -> Type
 type pkey (p:(text -> Type)) = k:key{key_prop k == p}
 
-assume val leak: k:key { forall t. key_prop k t } -> bytes 
-assume val leaked: k:key -> b:bool { b ==> (forall t. key_prop k t) }   
+assume val leak: k:key { forall t. key_prop k t } -> bytes
+assume val leaked: k:key -> b:bool { b ==> (forall t. key_prop k t) }
 
 (* this function returns the key bytes, and marks the key as corrupted *)
 
@@ -57,34 +60,33 @@ assume val keygen: p:(text -> Type) -> pkey p
 val mac:    k:key -> t:text{key_prop k t} -> tag
 val verify: k:key -> t:text -> tag -> b:bool{b ==> key_prop k t}
 
-(* to model authentication, we log all genuine calls to MACs *) 
+(* to model authentication, we log all genuine calls to MACs *)
 
 (* the ideal implementation below uses a global log *)
 
-type entry = 
+type entry =
   | Entry : k:key
          -> t:text{key_prop k t}
          -> m:tag
          -> entry
 
-let log = ST.alloc #(list entry) [] 
+let log = ST.alloc #(list entry) []
 
-let mac k t = 
+let mac k t =
   let m = sha1 k t in
   log := Entry k t m :: !log;
   m
 
 let verify k text tag =
-  let verified = sha1verify k text tag in 
-  let found    = is_Some(List.find (function (Entry k' text' tag') -> k=k' && text=text' (*CTXT: && tag=tag' *) ) !log) in 
+  let verified = sha1verify k text tag in
+  let found    = is_Some(List.find (function (Entry k' text' tag') -> k=k' && text=text' (*CTXT: && tag=tag' *) ) !log) in
 
-  (* plain, concrete implementation (ignoring the log) *) 
-//verified           
+  (* plain, concrete implementation (ignoring the log) *)
+//verified
 
-  (* ideal, error-correcting implementation *) 
-  verified && (found || leaked k ) 
+  (* ideal, error-correcting implementation *)
+  verified && (found || leaked k )
 
   (* error-detecting implementation for the INT-CMA-LEAK game *)
 //if verified && not (found || leaked k) then win:= Some(k,text,tag);
-//verified 
-
+//verified
